Add the inst io_acts as parameter to the source context

io/Compiler.Model.fst
@@ -12,27 +12,53 @@ open TC.Monitorable.Hist
 open Compiler.Languages
 open Compile.IIO.To.ILang
 
+type typ_io_cmds (fl:erased tflag) (pi:monitorable_prop) =
+  (cmd : io_cmds) ->
+  (arg : io_sig.args cmd) ->
+  IIO (io_sig.res cmd arg) fl
+    (requires (fun _ -> True))
+    (ensures (fun h r lt ->
+      (match r with
+       | Inr Contract_failure -> ~(pi cmd arg h) /\ lt == []
+       | r' -> pi cmd arg h /\ lt == [convert_call_to_event cmd arg r'])))
+
+val inst_io_cmds : pi:monitorable_prop -> typ_io_cmds AllActions pi
+let inst_io_cmds pi cmd arg =
+  let h = get_trace () in
+  if pi cmd arg h then (admit (); static_cmd cmd arg)
+  else Inr Contract_failure
+
+(**
+val convert_insts : (ipi:monitorable_prop) -> (epi:monitorable_prop) -> (_:squash (forall h cmd arg. epi cmd arg h ==> ipi cmd arg h)) ->
+  (cmd_call:typ_io_cmds AllActions ipi) -> (typ_io_cmds AllActions epi) 
+let convert_insts ipi epi () cmd_call cmd arg = 
+  assert (forall h. epi cmd arg h ==> ipi cmd arg h);
+  cmd_call cmd arg 
+**)
+
 (** *** IIO interface **)
 noeq
 type iio_interface = {
-  pt : Type;
   ct : erased tflag -> Type;
+  pt : Type;
 
-  ct_rc : tree pck_rc;
-  pt_rc : tree pck_rc;
+  ct_rcs : tree pck_rc;
+  //pt_rc : tree pck_rc;
 
-  ipi : monitorable_prop;
+  epi : monitorable_prop;
+ // ipi : monitorable_prop;
+//  ipi_stronger_epi : squash (forall h cmd arg. ipi cmd arg h ==> epi cmd arg h);
 
-  pt_exportable : exportable pt ipi pt_rc AllActions;
-  ct_importable : fl:erased tflag -> importable (ct fl) ipi ct_rc fl;
+  //pt_exportable : exportable pt ipi pt_rc AllActions;
+  ct_importable : fl:erased tflag -> importable (ct fl) epi ct_rcs fl;
 }
 
-let make_all_rc_eff (rcs:tree pck_rc) : typ_posts AllActions rcs =
+let make_rcs_eff (rcs:tree pck_rc) : typ_posts AllActions rcs =
   let r : tree (pck_eff_rc AllActions) = map_tree rcs make_rc_eff in
   assume (equal_trees rcs (map_tree r dfst));
   r
 
-type ctx_iio (i:iio_interface) = #fl:erased tflag -> typ_posts fl i.ct_rc -> i.ct fl 
+type ctx_iio (i:iio_interface) = #fl:erased tflag -> typ_posts fl i.ct_rcs -> typ_io_cmds fl i.epi -> i.ct fl 
 
 type prog_iio (i:iio_interface) = i.ct AllActions -> i.pt
 
@@ -44,8 +70,8 @@ let iio_language : language = {
   whole = (i:iio_interface & i.pt);
 
   link = (fun #i p c -> 
-    let eff_rc = make_all_rc_eff i.ct_rc in
-    (| i, p (c #AllActions eff_rc) |));
+    let eff_rcs = make_rcs_eff i.ct_rcs in
+    (| i, p (c #AllActions eff_rcs (inst_io_cmds i.epi)) |));
   event_typ = IO.Sig.event;
 
   beh = admit ()
@@ -57,10 +83,10 @@ type ilang_interface = {
   pt : Type;
   ct : erased tflag -> Type;
 
-  ipi : monitorable_prop;
+  epi : monitorable_prop;
   
-  pt_ilang : ilang pt ipi;
-  ct_ilang : fl:erased tflag -> ilang (ct fl) ipi;
+  //pt_ilang : ilang pt ipi;
+  ct_ilang : fl:erased tflag -> ilang (ct fl) epi;
 }
 
 type ctx_ilang (i:ilang_interface) = #fl:erased tflag -> i.ct fl
@@ -81,11 +107,12 @@ let ilang_language : language = {
 
 (** ** Compile interfaces **)
 let comp_int_iio_ilang (i:iio_interface) : ilang_interface = {
-  pt = resexn i.pt_exportable.etype;
+ // pt = resexn i.pt_exportable.etype;
+  pt = resexn i.pt;
   ct = (fun fl -> (i.ct_importable fl).itype);
-  ipi = i.ipi;
+  epi = i.epi;
 
-  pt_ilang = ilang_resexn i.ipi i.pt_exportable.etype #i.pt_exportable.c_etype;
+//  pt_ilang = ilang_resexn i.ipi i.pt_exportable.etype #i.pt_exportable.c_etype;
   ct_ilang = (fun fl -> (i.ct_importable fl).c_itype);
 }
 
@@ -93,12 +120,13 @@ let comp_int_iio_ilang (i:iio_interface) : ilang_interface = {
 (** ** Phases of compilation **)
 let compiler_pprog_iio_ilang (#i:iio_interface) (p_s:prog_iio i) : ilang_language.pprog (comp_int_iio_ilang i) = 
   fun c_t -> 
-    let eff_rc = make_all_rc_eff i.ct_rc in
+    let eff_rc = make_rcs_eff i.ct_rcs in
     match (i.ct_importable AllActions).import c_t eff_rc with
     | Inl (c_s:i.ct AllActions) -> begin
        let p : i.pt = p_s c_s in
-       let eff_rc = make_all_rc_eff i.pt_rc in
-       Inl (i.pt_exportable.export eff_rc p)
+       // let eff_rc = make_all_rc_eff i.pt_rc in
+       // Inl (i.pt_exportable.export eff_rc p)
+       Inl p
     end
     | Inr err -> Inr err
 
@@ -117,20 +145,24 @@ open FStar.List
 
 (** Tests **)
 let test_interface : iio_interface = {
-  ipi = (fun _ _ _ -> true);
+  epi = (fun _ _ _ -> true);
 
-  pt = unit -> IIOpi (resexn unit) AllActions (fun _ _ _ -> true);
-  pt_rc = EmptyNode Leaf Leaf;
+  pt = unit -> IIO (resexn unit) AllActions (fun _ -> True) (fun _ _ _ -> true);
+  // pt_rc = EmptyNode Leaf Leaf;
 
   ct = (fun fl -> unit -> IIO (resexn file_descr) fl (fun _ -> True) (fun h rfd lt -> Inl? rfd ==> is_open (Inl?.v rfd) (rev lt @ h)));
-  ct_rc = Node (| unit, resexn file_descr, (fun () h (rfd:resexn file_descr) lt -> Inl? rfd && (is_open (Inl?.v rfd) (rev lt @ h))) |) Leaf Leaf;
+  ct_rcs = Node (| unit, resexn file_descr, (fun () h (rfd:resexn file_descr) lt -> Inl? rfd && (is_open (Inl?.v rfd) (rev lt @ h))) |) Leaf Leaf;
 
 
-  pt_exportable = exportable_arrow_with_no_pre_and_no_post unit #importable_unit unit #exportable_unit;
+  // pt_exportable = exportable_arrow_with_no_pre_and_no_post unit #importable_unit unit #exportable_unit;
   ct_importable = admit () //safe_importable_is_importable (safe_importable_arrow_pre_post file_descr unit );
 }
 
 val test_prog : prog_iio test_interface
-let test_prog ctx () : IIOpi (resexn unit) AllActions (fun _ _ _ -> true) by (unfold_def (`pi_as_hist); unfold_def (`hist_return); explode (); bump_nth 3; dump "H") =
+let test_prog ctx () : IIO (resexn unit) AllActions (fun _ -> True) (fun _ _ _ -> True) =
   let _ = ctx () in
   Inl ()
+
+val test_ctx : ctx_iio test_interface
+let test_ctx #fl eff_rcs io_acts () : IIO (resexn file_descr) fl (fun _ -> True) (fun h rfd lt -> Inl? rfd ==> is_open (Inl?.v rfd) (rev lt @ h)) = 
+  io_acts Openfile "/etc/passwd"
